src/Bedrock/Group/ScalarMult/MontgomeryLadder.v
@@ -5,11 +5,11 @@ Require Import Rupicola.Lib.ControlFlow.CondSwap.
 Require Import Rupicola.Lib.ControlFlow.DownTo.
 Require Import Crypto.Arithmetic.PrimeFieldTheorems.
 Require Import Crypto.Bedrock.Group.ScalarMult.LadderStep.
-Require Import Crypto.Bedrock.ScalarField.Interface.Compilation.
 Require Import Crypto.Bedrock.Specs.Field.
-Require Import Crypto.Bedrock.Specs.ScalarField.
 Require Import Crypto.Util.NumTheoryUtil.
 Require Import Crypto.Bedrock.Field.Interface.Compilation2.
+
+Require bedrock2.NotationsCustomEntry. Import bedrock2.Syntax.Coercions.
 
 Require Import bedrock2.ZnWords.
 
@@ -40,8 +40,38 @@ Notation "'let/n' ( v , w , x , y , z ) := val 'in' body" :=
     (at level 200, v ident, w ident, x ident, y ident, z ident, body at level 200,
      only parsing).
 
+Section Gallina.
+  Local Open Scope F_scope.
+  Definition montladder_gallina (m : positive) (a24 : F m) (count : nat) (k : Z) (u : F m)
+    : F m :=
+    let/n X1 := stack 1 in
+    let/n Z1 := stack 0 in
+    let/n X2 := stack u in
+    let/n Z2 := stack 1 in
+    let/n swap := false in
+    let/n (X1, Z1, X2, Z2, swap) :=
+       downto
+         \<X1, Z1, X2, Z2, swap\> (* initial state *)
+         count
+         (fun state i =>
+            let '\<X1, Z1, X2, Z2, swap\> := state in
+            let/n s_i := Z.testbit k (Z.of_nat i) in
+            let/n swap := xorb swap s_i in
+            let/n (X1, X2) := cswap swap X1 X2 in
+            let/n (Z1, Z2) := cswap swap Z1 Z2 in
+            let/n (X1, Z1, X2, Z2) := ladderstep_gallina m a24 u X1 Z1 X2 Z2 in
+            let/n swap := s_i in
+            \<X1, Z1, X2, Z2, swap\>
+         ) in
+    let/n (X1, X2) := cswap swap X1 X2 in
+    let/n (Z1, Z2) := cswap swap Z1 Z2 in
+    let/n OUT := (F.inv Z1) in
+    let/n OUT := (X1 * OUT) in
+    OUT.
+End Gallina.
 
 Section __.
+
   Context {width: Z} {BW: Bitwidth width} {word: word.word width} {mem: map.map word Byte.byte}.
   Context {locals: map.map String.string word}.
   Context {env: map.map String.string (list String.string * list String.string * Syntax.cmd)}.
@@ -50,68 +80,30 @@ Section __.
   Context {locals_ok : map.ok locals}.
   Context {env_ok : map.ok env}.
   Context {ext_spec_ok : Semantics.ext_spec.ok ext_spec}.
-  Context {field_parameters : FieldParameters}
-          {scalar_field_parameters : ScalarFieldParameters}.
-  Context {scalar_field_parameters_ok : ScalarFieldParameters_ok}.
-  Context {field_representaton : FieldRepresentation}
-          {scalar_representation : ScalarRepresentation}.
+  Context {field_parameters : FieldParameters}.
+  Context {field_representaton : FieldRepresentation}.
   Context {field_representation_ok : FieldRepresentation_ok}.
   Hint Resolve @relax_bounds : compiler.
 
-  Section Gallina.
-    Local Open Scope F_scope.
-
-    Definition montladder_gallina
-               (scalarbits : Z) (testbit:nat ->bool) (u:F M_pos)
-      : F M_pos :=
-      let/n X1 := stack 1 in
-      let/n Z1 := stack 0 in
-      let/n X2 := stack u in
-      let/n Z2 := stack 1 in
-      let/n swap := false in
-      let/n count := scalarbits in
-      let/n (X1, Z1, X2, Z2, swap) :=
-         downto
-           \<X1, Z1, X2, Z2, swap\> (* initial state *)
-           (Z.to_nat count)
-           (fun state i =>
-              let '\<X1, Z1, X2, Z2, swap\> := state in
-              let/n s_i := testbit i in
-              let/n swap := xorb swap s_i in
-              let/n (X1, X2) := cswap swap X1 X2 in
-              let/n (Z1, Z2) := cswap swap Z1 Z2 in
-              let/n (X1, Z1, X2, Z2) := ladderstep_gallina u X1 Z1 X2 Z2 in
-              let/n swap := s_i in
-              \<X1, Z1, X2, Z2, swap\>
-           ) in
-      let/n (X1, X2) := cswap swap X1 X2 in
-      let/n (Z1, Z2) := cswap swap Z1 Z2 in
-      let/n OUT := (F.inv Z1) in
-      let/n OUT := (X1 * OUT) in
-      OUT.
-  End Gallina.
-
   Section MontLadder.
-    Context (scalarbits_small : word.wrap scalarbits = scalarbits).
+    Context scalarbits (scalarbits_small : word.wrap (Z.of_nat scalarbits) = Z.of_nat scalarbits).
+    Local Notation "bs $@ a" := (array ptsto (word.of_Z 1) a bs) (at level 20).
 
     Instance spec_of_montladder : spec_of "montladder" :=
       fnspec! "montladder"
             (pOUT pK pU : word)
-            / (K : scalar) (U : F M_pos) (* inputs *)
+            / Kbytes (K : Z) (U : F M_pos) (* inputs *)
             out_bound OUT
             R,
       { requires tr mem :=
-          (FElem out_bound pOUT OUT * Scalar pK K * FElem (Some tight_bounds) pU U
+          LittleEndianList.le_combine Kbytes = K /\
+          Z.of_nat scalarbits <= 8*Z.of_nat (length Kbytes) /\
+          (FElem out_bound pOUT OUT * Kbytes$@pK * FElem (Some tight_bounds) pU U
            *  R)%sep mem;
         ensures tr' mem' :=
           tr' = tr
-          /\ (let OUT := montladder_gallina
-                           scalarbits
-                           (fun i =>
-                              Z.testbit (F.to_Z (sceval K))
-                                        (Z.of_nat i))
-                           U in
-              (FElem (Some tight_bounds) pOUT OUT * Scalar pK K
+          /\ (let OUT := montladder_gallina M_pos a24 scalarbits K U in
+              (FElem (Some tight_bounds) pOUT OUT * Kbytes$@pK
                * FElem (Some tight_bounds) pU U
                * R)%sep mem') }.
 
@@ -124,194 +116,245 @@ Section __.
     Lemma unsigned_of_Z_0 : word.unsigned (@word.of_Z _ word 0) = 0.
     Proof. exact word.unsigned_of_Z_0. Qed.
     Hint Resolve unsigned_of_Z_0 unsigned_of_Z_1 : compiler.
+    Import bedrock2.NotationsCustomEntry.
+ Lemma compile_sctestbit : forall {tr mem locals functions} bs x i,
+   let v := Z.testbit x (Z.of_nat i) in
+   forall {P} {pred: P v -> predicate} {k: nlet_eq_k P v} {k_impl}
+     R x_ptr x_var wi i_var out_var,
 
-    
-    Existing Instance spec_of_sctestbit.
-    
-    Hint Extern 8
-         (WeakestPrecondition.cmd _ _ _ _ _ (_ (nlet_eq _ (Z.testbit (F.to_Z (sceval _)) _) _))) =>
-    simple eapply compile_sctestbit; shelve : compiler.
+     (bs$@x_ptr * R)%sep mem ->
+     map.get locals x_var = Some x_ptr ->
 
+     LittleEndianList.le_combine bs = x ->
 
-    (*TODO: determine the best place for felem_cswap. Should it get its own file?*)
-    Definition felem_cswap := "felem_cswap".
-    (*TODO: move to the right place;
-    TODO: instantiate
-     *)  
-    Instance spec_of_felem_cswap : spec_of felem_cswap :=
-      fnspec! felem_cswap mask ptr1 ptr2 / b1 b2 b c1 c2 R,
-      { requires tr mem :=
-          mask = word.of_Z (Z.b2z b) /\
-          (FElem b1 ptr1 c1 * FElem b2 ptr2 c2 * R)%sep mem;
-        ensures tr' mem' :=
-          tr' = tr /\
-          let (c1,c2) := cswap b c1 c2 in
-          let (b1,b2) := cswap b b1 b2 in
-          (FElem b1 ptr1 c1 * FElem b2 ptr2 c2 * R)%sep mem' }.
-    
-    Lemma compile_felem_cswap {tr m l functions} swap (lhs rhs : F M_pos) :
-      let v := cswap swap lhs rhs in
-      forall {P} {pred: P v -> predicate} {k: nlet_eq_k P v} {k_impl}
-             R mask_var lhs_ptr lhs_var b_lhs rhs_ptr rhs_var b_rhs,
+     wi = word.of_Z (Z.of_nat i) ->
+     Z.of_nat i < 8 * Z.of_nat (length bs) ->
+     map.get locals i_var = Some wi ->
 
-        spec_of_felem_cswap functions ->
-
-        map.get l mask_var = Some (word.of_Z (Z.b2z swap)) ->
-        
-        map.get l lhs_var = Some lhs_ptr ->
-        map.get l rhs_var = Some rhs_ptr ->
-
-        (FElem b_lhs lhs_ptr lhs * FElem b_rhs rhs_ptr rhs * R)%sep m ->
-
-        (let v := v in
-         let (b1,b2) := cswap swap b_lhs b_rhs in
-         forall m',
-           (FElem b1 lhs_ptr (fst v) * FElem b2 rhs_ptr (snd v) * R)%sep m' ->
-           (<{ Trace := tr;
-               Memory := m';
-               Locals := l;
-               Functions := functions }>
-            k_impl
-            <{ pred (k v eq_refl) }>)) ->
-        <{ Trace := tr;
-           Memory := m;
-           Locals := l;
-           Functions := functions }>
-        cmd.seq
-          (cmd.call [] felem_cswap [expr.var mask_var; expr.var lhs_var; expr.var rhs_var])
-          k_impl
-        <{ pred (nlet_eq [lhs_var; rhs_var] v k) }>.
-    Proof.     
-      Local Ltac prove_field_compilation locals :=
-        repeat straightline' locals;
-        handle_call;
-        lazymatch goal with
-        | |- sep _ _ _ => ecancel_assumption
-        | _ => idtac
-        end; eauto;
-        sepsimpl; repeat straightline' locals; subst; eauto.
-      prove_field_compilation l.
-      destruct swap; eapply H4; unfold v; unfold cswap; simpl; eauto.
-    Qed.
-    Hint Resolve compile_felem_cswap : compiler.
-
-    Existing Instance felem_alloc.
-
-
-    Lemma cswap_same {A} b (a : A): cswap b a a = (a,a).
-    Proof.
-      destruct b; reflexivity.
-    Qed.
-    
-    Local Ltac ecancel_assumption ::= ecancel_assumption_impl.
-
-    Lemma scalarbits_bound : scalarbits < 2 ^ width.
-    Proof.
-      rewrite <- scalarbits_small.
-      unfold word.wrap.
-      apply Z_mod_lt.
-      pose proof word.width_pos.
-      pose proof (Z.pow_pos_nonneg 2 width ltac:(lia)).
-      lia.
-    Qed.
-
-    (* TODO: why doesn't `Existing Instance` work?
-    Existing Instance spec_of_sctestbit.*)
-    Hint Extern 1 (spec_of sctestbit) =>
-    (simple refine (@spec_of_sctestbit _ _ _ _ _ _ _ _)) : typeclass_instances.
-    Hint Extern 1 (spec_of "ladderstep") =>
-    (simple refine (@spec_of_ladderstep _ _ _ _ _ _ _ _)) : typeclass_instances.
-
-    (* TODO: this seems a bit delicate*)
-    Ltac compile_cswap :=
-      eapply compile_felem_cswap;
-      [solve[repeat compile_step] ..
-      | repeat compile_step;
-        rewrite cswap_same;
-        compile_step;      
-        match goal with
-        | [|- (WeakestPrecondition.cmd _ _ _ _ _ (_ (let (_,_) := ?v in _)))] =>
-          destruct v
-        end].
-    
-    Hint Extern 8 (WeakestPrecondition.cmd _ _ _ _ _ (_ (nlet_eq _ (cswap _ _ _) _))) =>
-    compile_cswap; shelve : compiler.
-    
-    
-    Lemma word_unsigned_of_Z_eq z
-      : 0 <= z < 2 ^ width -> word.unsigned (word.of_Z z : word) = z.
-    Proof.
-      intros.
-      rewrite word.unsigned_of_Z.
-      rewrite word.wrap_small; auto.
-    Qed.
-
-    Hint Extern 8 (word.unsigned (word.of_Z _) = _) =>
-    simple eapply word_unsigned_of_Z_eq; [ ZnWords |] : compiler.
-
-    (*TODO: should this go in core rupicola?*)
-    Lemma compile_copy_bool {tr m l functions} (x: bool) :
-      let v := x in
-      forall {P} {pred: P v -> predicate}
-             {k: nlet_eq_k P v} {k_impl}
-             x_expr var,
-
-        WeakestPrecondition.dexpr m l x_expr (word.of_Z (Z.b2z v)) ->
-
-        (let v := v in
-         <{ Trace := tr;
-            Memory := m;
-            Locals := map.put l var (word.of_Z (Z.b2z v));
+     (let v := v in
+        (<{ Trace := tr;
+            Memory := mem;
+            Locals := map.put locals out_var (word.b2w v);
             Functions := functions }>
          k_impl
-         <{ pred (k v eq_refl) }>) ->
-        <{ Trace := tr;
-           Memory := m;
-           Locals := l;
-           Functions := functions }>
-        cmd.seq (cmd.set var x_expr) k_impl
-        <{ pred (nlet_eq [var] v k) }>.
-    Proof.
-      intros.
-      repeat straightline.
-      eauto.
-    Qed.
-    Hint Extern 10 (WeakestPrecondition.cmd _ _ _ _ _ (_ (nlet_eq _ ?v _))) =>
-    is_var v; simple eapply compile_copy_bool; shelve : compiler.
+         <{ pred (k v eq_refl) }>)) ->
+     <{ Trace := tr;
+        Memory := mem;
+        Locals := locals;
+        Functions := functions }>
+     bedrock_cmd:(out_var = (load1(x_var+i_var>>coq:(3))>>(i_var&coq:(7)))&coq:(1); coq:(k_impl))
+     <{ pred (nlet_eq [out_var] v k) }>.
+ Proof.
+   repeat straightline.
+   repeat (eexists; split; repeat straightline'; eauto); cbn; repeat straightline.
+
+   eapply load_one_of_sep.
+   (*
+     (* Note: could instead add the following two lines to seprewrite0_in but kinda wanna avoid reduction/conversion there...  *)
+    let t := type of Hrw in
+    let t := eval cbv zeta in t in
+    *)
+   let Hrw := open_constr:(@bytearray_index_inbounds _ _ _ _ _ _ _ _ _ : Lift1Prop.iff1 _ _) in
+   seprewrite0_in Hrw H; ecancel_assumption.
+
+   unfold word.b2w.
+   subst_lets_in_goal; subst.
+   eapply word.unsigned_inj; repeat rewrite
+     ?word.unsigned_of_Z, ?word.unsigned_and_nowrap, ?word.unsigned_sru_nowrap.
+   all : cbv [word.wrap]; rewrite ?Z.mod_small.
+   all : change 7 with (Z.ones 3); change 1 with (Z.ones 1); rewrite ?Z.land_ones.
+   all : rewrite ?Z.shiftr_div_pow2; change (2^3) with 8; change (2^1) with 2.
+   all : rewrite <-?hd_skipn_nth_default.
+   rewrite <-Z.testbit_spec'; f_equal.
+   replace (Z.to_nat (Z.of_nat i / 8)) with (i/8)%nat.
+   all : try (destruct Bitwidth.width_cases; cbn; Lia.lia).
+   (* word<->Z side conditions and nth_default le_combine
+      Z.testbit (LittleEndianList.le_combine bs) (Z.of_nat i) =
+      Z.testbit (byte.unsigned (nth_default (byte.of_Z 0) bs (i / 8))) (Z.of_nat i mod 8)
+    *)
+ Admitted.
+
+  Hint Extern 8
+       (WeakestPrecondition.cmd _ _ _ _ _ (_ (nlet_eq _ (Z.testbit _ _) _))) =>
+  simple eapply compile_sctestbit; shelve : compiler.
 
 
-    Hint Resolve unsigned_of_Z_0 : compiler_side_conditions.
-    Hint Resolve unsigned_of_Z_1 : compiler_side_conditions.
-    Hint Unfold F.one F.zero : compiler_cleanup.
+  (*TODO: determine the best place for felem_cswap. Should it get its own file?*)
+  Definition felem_cswap := "felem_cswap".
+  (*TODO: move to the right place;
+  TODO: instantiate
+   *)  
+  Instance spec_of_felem_cswap : spec_of felem_cswap :=
+    fnspec! felem_cswap mask ptr1 ptr2 / b1 b2 b c1 c2 R,
+    { requires tr mem :=
+        mask = word.of_Z (Z.b2z b) /\
+        (FElem b1 ptr1 c1 * FElem b2 ptr2 c2 * R)%sep mem;
+      ensures tr' mem' :=
+        tr' = tr /\
+        let (c1,c2) := cswap b c1 c2 in
+        let (b1,b2) := cswap b b1 b2 in
+        (FElem b1 ptr1 c1 * FElem b2 ptr2 c2 * R)%sep mem' }.
+  
+  Lemma compile_felem_cswap {tr m l functions} swap (lhs rhs : F M_pos) :
+    let v := cswap swap lhs rhs in
+    forall {P} {pred: P v -> predicate} {k: nlet_eq_k P v} {k_impl}
+           R mask_var lhs_ptr lhs_var b_lhs rhs_ptr rhs_var b_rhs,
 
-    Hint Extern 10 (_ < _) => lia : compiler_side_conditions.
+      spec_of_felem_cswap functions ->
 
-    (* TODO: update the original definition in bedrock2 *)
-    Ltac find_implication xs y ::=
-      multimatch xs with
-      | cons ?x _ =>
-          (* Only proceed if we can find an implication between x and y *)
-          let _ := constr:(ltac:(solve [auto 1 with nocore ecancel_impl])
-                            : Lift1Prop.impl1 x y) in
-          constr:(O)
-      | cons _ ?xs => let i := find_implication xs y in constr:(S i)
-      end.
-    
-    Derive montladder_body SuchThat
-           (defn! "montladder" ("OUT", "K", "U")
-                { montladder_body },
-             implements montladder_gallina
-                        using [felem_cswap; felem_copy; felem_small_literal;
-                               sctestbit; "ladderstep"; inv; mul])
-           As montladder_correct.
-    Proof.
-      pose proof scalarbits_pos.
-      pose proof scalarbits_bound.
-      compile_setup;
-      solve[repeat repeat compile_step];
-      compile_done.
-    Qed.
-  End MontLadder.
+      map.get l mask_var = Some (word.of_Z (Z.b2z swap)) ->
+      
+      map.get l lhs_var = Some lhs_ptr ->
+      map.get l rhs_var = Some rhs_ptr ->
+
+      (FElem b_lhs lhs_ptr lhs * FElem b_rhs rhs_ptr rhs * R)%sep m ->
+
+      (let v := v in
+       let (b1,b2) := cswap swap b_lhs b_rhs in
+       forall m',
+         (FElem b1 lhs_ptr (fst v) * FElem b2 rhs_ptr (snd v) * R)%sep m' ->
+         (<{ Trace := tr;
+             Memory := m';
+             Locals := l;
+             Functions := functions }>
+          k_impl
+          <{ pred (k v eq_refl) }>)) ->
+      <{ Trace := tr;
+         Memory := m;
+         Locals := l;
+         Functions := functions }>
+      cmd.seq
+        (cmd.call [] felem_cswap [expr.var mask_var; expr.var lhs_var; expr.var rhs_var])
+        k_impl
+      <{ pred (nlet_eq [lhs_var; rhs_var] v k) }>.
+  Proof.     
+    Local Ltac prove_field_compilation locals :=
+      repeat straightline' locals;
+      handle_call;
+      lazymatch goal with
+      | |- sep _ _ _ => ecancel_assumption
+      | _ => idtac
+      end; eauto;
+      sepsimpl; repeat straightline' locals; subst; eauto.
+    prove_field_compilation l.
+    destruct swap; eapply H4; unfold v; unfold cswap; simpl; eauto.
+  Qed.
+  Hint Resolve compile_felem_cswap : compiler.
+
+  Existing Instance felem_alloc.
+
+
+  Lemma cswap_same {A} b (a : A): cswap b a a = (a,a).
+  Proof.
+    destruct b; reflexivity.
+  Qed.
+  
+  Local Ltac ecancel_assumption ::= ecancel_assumption_impl.
+
+  Lemma scalarbits_bound : Z.of_nat scalarbits < 2 ^ width.
+  Proof.
+    rewrite <- scalarbits_small.
+    unfold word.wrap.
+    apply Z_mod_lt.
+    pose proof word.width_pos.
+    pose proof (Z.pow_pos_nonneg 2 width ltac:(lia)).
+    lia.
+  Qed.
+
+  (* TODO: why doesn't `Existing Instance` work?
+  Existing Instance spec_of_sctestbit.*)
+  Hint Extern 1 (spec_of "ladderstep") =>
+  (simple refine (@spec_of_ladderstep _ _ _ _ _ _ _ _)) : typeclass_instances.
+
+  (* TODO: this seems a bit delicate*)
+  Ltac compile_cswap :=
+    eapply compile_felem_cswap;
+    [solve[repeat compile_step] ..
+    | repeat compile_step;
+      rewrite cswap_same;
+      compile_step;      
+      match goal with
+      | [|- (WeakestPrecondition.cmd _ _ _ _ _ (_ (let (_,_) := ?v in _)))] =>
+        destruct v
+      end].
+  
+  Hint Extern 8 (WeakestPrecondition.cmd _ _ _ _ _ (_ (nlet_eq _ (cswap _ _ _) _))) =>
+  compile_cswap; shelve : compiler.
+  
+  
+  Lemma word_unsigned_of_Z_eq z
+    : 0 <= z < 2 ^ width -> word.unsigned (word.of_Z z : word) = z.
+  Proof.
+    intros.
+    rewrite word.unsigned_of_Z.
+    rewrite word.wrap_small; auto.
+  Qed.
+
+  Hint Extern 8 (word.unsigned (word.of_Z _) = _) =>
+  simple eapply word_unsigned_of_Z_eq; [ ZnWords |] : compiler.
+
+  (*TODO: should this go in core rupicola?*)
+  Lemma compile_copy_bool {tr m l functions} (x: bool) :
+    let v := x in
+    forall {P} {pred: P v -> predicate}
+           {k: nlet_eq_k P v} {k_impl}
+           x_expr var,
+
+      WeakestPrecondition.dexpr m l x_expr (word.of_Z (Z.b2z v)) ->
+
+      (let v := v in
+       <{ Trace := tr;
+          Memory := m;
+          Locals := map.put l var (word.of_Z (Z.b2z v));
+          Functions := functions }>
+       k_impl
+       <{ pred (k v eq_refl) }>) ->
+      <{ Trace := tr;
+         Memory := m;
+         Locals := l;
+         Functions := functions }>
+      cmd.seq (cmd.set var x_expr) k_impl
+      <{ pred (nlet_eq [var] v k) }>.
+  Proof.
+    intros.
+    repeat straightline.
+    eauto.
+  Qed.
+  Hint Extern 10 (WeakestPrecondition.cmd _ _ _ _ _ (_ (nlet_eq _ ?v _))) =>
+  is_var v; simple eapply compile_copy_bool; shelve : compiler.
+
+
+  Hint Resolve unsigned_of_Z_0 : compiler_side_conditions.
+  Hint Resolve unsigned_of_Z_1 : compiler_side_conditions.
+  Hint Unfold F.one F.zero : compiler_cleanup.
+
+  Hint Extern 10 (_ < _) => lia : compiler_side_conditions.
+
+  (* TODO: update the original definition in bedrock2 *)
+  Ltac find_implication xs y ::=
+    multimatch xs with
+    | cons ?x _ =>
+        (* Only proceed if we can find an implication between x and y *)
+        let _ := constr:(ltac:(solve [auto 1 with nocore ecancel_impl])
+                          : Lift1Prop.impl1 x y) in
+        constr:(O)
+    | cons _ ?xs => let i := find_implication xs y in constr:(S i)
+    end.
+  
+  Derive montladder_body SuchThat
+         (defn! "montladder" ("OUT", "K", "U")
+              { montladder_body },
+           implements montladder_gallina
+                      using [felem_cswap; felem_copy; felem_small_literal;
+                             "ladderstep"; inv; mul])
+         As montladder_correct.
+  Proof.
+    pose proof scalarbits_bound.
+    compile_setup;
+    repeat repeat compile_step.
+    all : try compile_done.
+  Qed.
+End MontLadder.
 End __.
 
 Global Hint Extern 1 (spec_of "montladder") => (simple refine (@spec_of_montladder _ _ _ _ _ _ _ _ _ _)) : typeclass_instances.
@@ -322,5 +365,7 @@ Local Unset Printing Coercions.
    Otherwise the build breaks.
  *)
 Local Set Printing Width 160.
-Redirect "Crypto.Bedrock.Group.ScalarMult.MontgomeryLadder.montladder_body" Print montladder_body.
-
+(*
+Import NotationsCustomEntry.
+*)
+Redirect "Crypto.Bedrock.Group.ScalarMult.MontgomeryLadder.montladder_body" Eval cbv [montladder_body cmd_downto_fresh cmd_downto gs fold_right] in montladder_body 253.
